verification/specs_general.v
@@ -1,153 +1,166 @@
 (** * General Specification of alloc functions
 
-Kathrin Stark, 2021. 
+Kathrin Stark, 2021.
 
-This file contains a general specification for the alloc function, 
-using a representation of constructors. 
- *)
+This file contains a general specification for the alloc function,
+using a representation of constructors.
+*)
 
-From VeriFFI Require Export library.base_representation. 
+From VeriFFI Require Export library.base_representation.
+From VeriFFI Require Export library.meta.
 From VeriFFI Require Export verification.graph_add.
-From VeriFFI Require Export verification.example.glue.
+(* From VeriFFI Require Export verification.example.glue. *)
 From VeriFFI Require Export verification.specs_library.
 
 
 (** ** 1. Representable Type Class
 
-A type representable in a graph consists of: 
-1. a type, X_type, which will be representable in the graph 
-2. a function, X_in_graph, which defines the representation in a graph 
-3. consistency conditions on X_in_graph, X_has_v and X_monotone, needed to actually get the later proof through: 
-   a. X_has_v: Whenever a node represents an element of X_type, then this node is present in the graph. 
+A type representable in a graph consists of:
+1. a type, X_type, which will be representable in the graph
+2. a function, X_in_graph, which defines the representation in a graph
+3. consistency conditions on X_in_graph, X_has_v and X_monotone, needed to actually get the later proof through:
+   a. X_has_v: Whenever a node represents an element of X_type, then this node is present in the graph.
    b. X_monotone: Adding (compatible) nodes to a graph doesn't change whether an element of a type is present in the graph.
  *)
 
-Record representable_X  := 
-  { X_type : Type; 
-    X_in_graph : graph -> X_type -> rep_type -> Prop;
-    X_has_v : forall g n v, X_in_graph g n (repNode v) -> graph_has_v g v;
-    X_monotone : forall g to lb e n p,
-        add_node_compatible g (new_copied_v g to) e 
-        -> graph_has_gen g to
-        -> X_in_graph g n p 
-        -> X_in_graph (add_node g to lb e) n p
-    }.
+(* Record representable_X  := *)
+(*   { X_type : Type; *)
+(*     X_in_graph : graph -> X_type -> rep_type -> Prop; *)
+(*     X_has_v : forall g n v, X_in_graph g n (repNode v) -> graph_has_v g v; *)
+(*     X_monotone : forall g to lb e n p, *)
+(*         add_node_compatible g (new_copied_v g to) e *)
+(*         -> graph_has_gen g to *)
+(*         -> X_in_graph g n p *)
+(*         -> X_in_graph (add_node g to lb e) n p *)
+(*     }. *)
 
-Existing Class representable_X.
+(* Existing Class representable_X. *)
 
 (** ** 2. Encoding constructors
 
-The code of a constructor which allows parameters, indices, dependent arguments 
-tailored to what we need for the specification. 
+The code of a constructor which allows parameters, indices, dependent arguments
+tailored to what we need for the specification.
 The representation uses a weak HOAS representation.
 See the examples section for more detailed examples.
 
 ARG is not strictly necessary as it is an instance of DEPARG, but simplifies the later representation.
- *) 
-
-Inductive constrCode :=
-(* the type parameters in parametric polymorphism, isn't represented immediately in memory,
-but the possibility for representation is needed later, e.g., A in [list A]
  *)
- | TYPEPARAM  : (representable_X -> constrCode) -> constrCode
-(* Non-type parameters of a fixed type which isn't represented in memory, e.g., n in [n < m] *)
- | PARAM  : forall X : Type, (X -> constrCode) -> constrCode
-(* index, represented in memory, e.g. the index of a vector *) 
- | INDEX  : forall (X_: representable_X), (X_type X_ -> constrCode) -> constrCode
- (* non-dependent version of arguments, argument represented in memory, e.g. for X/list X of cons *)
- | ARG : representable_X -> constrCode -> constrCode
- (* dependent argument, represented in memory, e.g. in positive_nat_list *)
- | DEPARG : forall (X_: representable_X), (X_type X_ -> constrCode) -> constrCode
-(* the end type, e.g., list X for cons : forall X, X -> list X -> **list X** *)
- | RES  : representable_X -> constrCode.
+
+(* Inductive constrCode := *)
+(* (* the type parameters in parametric polymorphism, isn't represented immediately in memory, *)
+(* but the possibility for representation is needed later, e.g., A in [list A] *)
+(*  *) *)
+(*  | TYPEPARAM  : (representable_X -> constrCode) -> constrCode *)
+(* (* Non-type parameters of a fixed type which isn't represented in memory, e.g., n in [n < m] *) *)
+(*  | PARAM  : forall X : Type, (X -> constrCode) -> constrCode *)
+(* (* index, represented in memory, e.g. the index of a vector *) *)
+(*  | INDEX  : forall (X_: representable_X), (X_type X_ -> constrCode) -> constrCode *)
+(*  (* non-dependent version of arguments, argument represented in memory, e.g. for X/list X of cons *) *)
+(*  | ARG : representable_X -> constrCode -> constrCode *)
+(*  (* dependent argument, represented in memory, e.g. in positive_nat_list *) *)
+(*  | DEPARG : forall (X_: representable_X), (X_type X_ -> constrCode) -> constrCode *)
+(* (* the end type, e.g., list X for cons : forall X, X -> list X -> **list X** *) *)
+(*  | RES  : representable_X -> constrCode. *)
 
 
 (** Representation of data needed for the argument part of an instance of a constrCodeuctor, e.g., in the with clause of a specification.
-This will be a dependent tuple. *) 
-Fixpoint args (c : constrCode) : Type :=
-    match c with 
-    | TYPEPARAM f => {X_ : representable_X & args (f X_) }
-    | PARAM X f => {x : X & args (f x) }
-    | INDEX X_ f => {x : X_type X_ & args (f x)}
-    | ARG X_ arg => (X_type X_ * args arg)%type
-    | DEPARG X_ f => {x : X_type X_ & args (f x) }
-    | RES x => unit
-end.
+This will be a dependent tuple. *)
+(* Fixpoint args (c : constrCode) : Type := *)
+(*     match c with *)
+(*     | TYPEPARAM f => {X_ : representable_X & args (f X_) } *)
+(*     | PARAM X f => {x : X & args (f x) } *)
+(*     | INDEX X_ f => {x : X_type X_ & args (f x)} *)
+(*     | ARG X_ arg => (X_type X_ * args arg)%type *)
+(*     | DEPARG X_ f => {x : X_type X_ & args (f x) } *)
+(*     | RES x => unit *)
+(* end. *)
 
-(* Instance of result type *) 
-Fixpoint getRes (c: constrCode) (xs : args c) : representable_X := 
-  match c as l return (args l -> representable_X) with
-  | TYPEPARAM f => fun H => let (X_, xs') := H in getRes (f X_) xs'
-  | PARAM X f => fun H => let (x, xs') := H in getRes (f x) xs'                                                                         
-  | INDEX X_ f => fun H => let (x, xs') := H in getRes (f x) xs'                                                                         
-  | ARG X_ arg => fun H => let (x, xs') := H in getRes arg xs'         
-  | DEPARG X_ f => fun H  => let (x, xs') := H in getRes (f x) xs'                                                    
-  | RES x => fun _ => x                                                                             
-  end xs.
+(* (* Instance of result type *) *)
+(* Fixpoint getRes (c: constrCode) (xs : args c) : representable_X := *)
+(*   match c as l return (args l -> representable_X) with *)
+(*   | TYPEPARAM f => fun H => let (X_, xs') := H in getRes (f X_) xs' *)
+(*   | PARAM X f => fun H => let (x, xs') := H in getRes (f x) xs' *)
+(*   | INDEX X_ f => fun H => let (x, xs') := H in getRes (f x) xs' *)
+(*   | ARG X_ arg => fun H => let (x, xs') := H in getRes arg xs' *)
+(*   | DEPARG X_ f => fun H  => let (x, xs') := H in getRes (f x) xs' *)
+(*   | RES x => fun _ => x *)
+(*   end xs. *)
 
-(** Full description of a constructor:
-   fitting identifier, the code for the constructor, 
-   and the corresponding Coq function for the constructor. 
+(* (** Full description of a constructor: *)
+(*    fitting identifier, the code for the constructor, *)
+(*    and the corresponding Coq function for the constructor. *)
 
-  This is what MetaCoq will have to generate.
- *) 
-Record constructor_description := 
-{ name : ident;
-  constr : constrCode; 
-  coqConstr : forall (xs : args constr), X_type (getRes constr xs)
-}.
+(*   This is what MetaCoq will have to generate. *)
+(*  *) *)
+(* Record constructor_description := *)
+(* { name : ident; *)
+(*   constr : constrCode; *)
+(*   coqConstr : forall (xs : args constr), X_type (getRes constr xs) *)
+(* }. *)
 
 (** ** 3. A General Specification *)
 
 (** Generation of the in_graphs predicate, given the constructor arguments. *)
-Fixpoint in_graphs (g : graph) (c: constrCode) (xs :args c) (ps : list rep_type) : Prop :=
-      match c as l return (args l -> Prop) with
-      | TYPEPARAM f => fun H => let (X_, xs') := H in in_graphs g (f X_) xs' ps
-      | PARAM X f => fun H => let (x, xs') := H in in_graphs g (f x) xs' ps                                                             
-      | INDEX X_ f => fun H => let (x, xs') := H in
-                          match ps with
-                          | [] => False
-                          | p :: ps' =>  X_in_graph X_ g x p  /\ in_graphs g (f x) xs' ps'
-                          end     
-      | ARG X_ arg => fun H : args (ARG X_ arg) =>
-                      let (x, xs') := H in
-                      match ps with
-                      | [] => False
-                      | p :: ps' => X_in_graph X_ g x p /\ in_graphs g arg xs' ps'
-                      end  
-     | DEPARG X_ f => fun H  => let (x, xs') := H in 
-                  match ps with
-                          | [] => False
-                          | p :: ps' =>  X_in_graph X_ g x p  /\ in_graphs g (f x) xs' ps'
-                          end                                                                             
-      | RES x => fun _ => ps = nil                                                                              
-      end xs.
+Fixpoint in_graphs
+         (g : graph) (c : reific Rep) (xs : args c) (ps : list rep_type) : Prop :=
+  match c as l return (args l -> Prop) with
+  | TYPEPARAM f =>
+      fun H => let (X_, xs') := H in
+               let (R_, xs') := xs' in
+        in_graphs g (f X_ R_) xs' ps
+  | PARAM X f =>
+      fun H => let (x, xs') := H in
+      in_graphs g (f x) xs' ps
+  | INDEX X_ R_ f =>
+      fun H => let (x, xs') := H in
+      match ps with
+      | [] => False
+      | p :: ps' =>  @is_in_graph X_ (@in_graph X_ R_) g x p /\ in_graphs g (f x) xs' ps'
+      end
+  | ARG X_ R_ arg =>
+      fun H (* : args (ARG X_ R_ arg) *) =>
+      let (x, xs') := H in
+      match ps with
+      | [] => False
+      | p :: ps' => @is_in_graph X_ (@in_graph X_ R_) g x p /\ in_graphs g arg xs' ps'
+      end
+  | DEPARG X_ R_ f =>
+      fun H  => let (x, xs') := H in
+      match ps with
+      | [] => False
+      | p :: ps' => @is_in_graph X_ (@in_graph X_ R_) g x p /\ in_graphs g (f x) xs' ps'
+      end
+  | RES x _ => fun _ => ps = nil
+  end xs.
 
-(** List of tulong depending on the number of arguments which are represented in memory, needed for the paramers *)
+(** List of [tulong] depending on the number of arguments
+    represented in memory, needed for the parameters. *)
+Fixpoint get_size (c : reific Rep) (xs : args c) : nat :=
+  match c as l return (args l -> nat) with
+  | TYPEPARAM f =>
+      fun H => let (X_, xs') := H in let (R_, xs') := xs' in get_size (f X_ R_) xs'
+  | PARAM X f =>
+      fun H => let (x, xs') := H in get_size (f x) xs'
+  | INDEX _ _ f =>
+      fun H => let (x, xs') := H in S (get_size (f x) xs')
+  | ARG _ X_ arg =>
+      fun H (* : args (ARG X_ arg) *) => let (x, xs') := H in S (get_size arg xs')
+  | DEPARG _ X_ f => fun H  => let (x, xs') := H in S (get_size (f x) xs')
+  | RES _ x => fun _ => O
+  end xs.
 
-Fixpoint get_size (c : constrCode) (xs : args c) : nat := 
-   match c as l return (args l -> nat) with
-      | TYPEPARAM f => fun H => let (X_, xs') := H in get_size (f X_) xs'
-      | PARAM X f => fun H => let (x, xs') := H in get_size (f x) xs'                                                         
-      | INDEX X_ f => fun H => let (x, xs') := H in S (get_size (f x) xs')    
-      | ARG X_ arg => fun H : args (ARG X_ arg) =>
-                      let (x, xs') := H in S (get_size arg xs')
-     | DEPARG X_ f => fun H  => let (x, xs') := H in S (get_size (f x) xs')                                                   
-      | RES x => fun _ => O                                                                            
-      end xs.
-
-Definition get_tulongs (c: constrCode) (xs: args c): list type :=
+Definition get_tulongs (c : reific Rep) (xs : args c) : list type :=
   repeat tulong (get_size c xs).
 
-Lemma in_graphs_size g c xs ps : 
-  in_graphs g c xs ps -> get_size c xs = length ps. 
+Lemma in_graphs_size (g : graph) (c : reific Rep) (xs : args c) (ps : list rep_type) :
+  in_graphs g c xs ps -> get_size c xs = length ps.
 Proof.
-  revert ps. induction c; simpl in *; intros; try (destruct xs); eauto. 
-  all: destruct ps; simpl; intuition eauto; congruence. 
+  revert ps.
+  induction c; simpl in *; intros; try (destruct xs); try (destruct s); eauto.
+  all: destruct ps; simpl; intuition eauto; try congruence.
 Qed.
 
-
-(** Custom notation with a list for PRE to make the specification better readable. *) 
+(** Custom notation with a list for PRE to make the specification better readable. *)
 Notation "'WITH'  x1 : t1 , x2 : t2 , x3 : t3 , x4 : t4 , x5 : t5 , x6 : t6 , x7 : t7 , x8 : t8 , x9 : t9 , x10 : t10 'PRE'  [[ xs ]] P 'POST' [ tz ] Q" :=
      (NDmk_funspec (xs, tz) cc_default (t1*t2*t3*t4*t5*t6*t7*t8*t9*t10)
            (fun x => match x with (x1,x2,x3,x4,x5,x6,x7,x8,x9,x10) => P%assert end)
@@ -157,321 +170,334 @@ Notation "'WITH'  x1 : t1 , x2 : t2 , x3 : t3 , x4 : t4 , x5 : t5 , x6 : t6 , x7
               x10 at level 0,
              P at level 100, Q at level 100) : funspec_scope.
 
-Definition alloc_make_spec_general (c : constructor_description) (n: nat) : ident * funspec :=
-DECLARE (name c)
-        WITH gv : globals, g : graph, ps : list rep_type, xs : args (constr c), roots : roots_t, sh : share, ti : val, outlier : outlier_t, f_info : fun_info, t_info : GCGraph.thread_info
-  PRE  [[ thread_info :: repeat tulong n ]]
-       PROP (n = get_size (constr c) xs;
-            in_graphs g _ xs ps;
-             writable_share sh
-             )
+Definition alloc_make_spec_general
+           (c : constructor_description)
+           (n : nat) : ident * funspec :=
+  DECLARE _w (* FIXME to actual C fn names somehow? *)
+    WITH gv : globals, g : graph, ps : list rep_type,
+         xs : args (ctor_reific c), roots : roots_t, sh : share,
+         ti : val, outlier : outlier_t, f_info : fun_info, t_info : GCGraph.thread_info
+    PRE  [[ thread_info :: repeat tulong n ]]
+       PROP (n = get_size (ctor_reific c) xs ;
+             in_graphs g _ xs ps ;
+             writable_share sh)
        (PARAMSx (ti :: map (fun p => rep_type_val g p) ps)
        (GLOBALSx nil
        (SEPx (full_gc g t_info roots outlier ti sh :: nil))))
-  POST [ tptr tulong  ]  
-     EX (p' : rep_type) (g' : graph) (t_info' : GCGraph.thread_info), 
-     PROP ( X_in_graph (getRes (constr c) xs) g' (coqConstr c xs) p'; 
-           gc_graph_iso g roots g' roots
-         ) 
-     RETURN  (rep_type_val g' p')
-     SEP (full_gc g' t_info' roots outlier ti sh).
+    POST [ tptr tulong ]
+      EX (p' : rep_type) (g' : graph) (t_info' : GCGraph.thread_info),
+        PROP (let r := result (ctor_reific c) xs in
+              @is_in_graph (projT1 r) (@in_graph (projT1 r) (projT2 r)) g' (ctor_real c xs) p' ;
+              gc_graph_iso g roots g' roots)
+        RETURN  (rep_type_val g' p')
+        SEP (full_gc g' t_info' roots outlier ti sh).
 
 
 
-(** ** 4. Examples *) 
+(** ** 4. Examples *)
 
-(** *** 4.0 Non-dependent, no indices/parameters - nat *)
+(* Require Import VeriFFI.generator.InGraph. *)
+(* Require Import VeriFFI.generator.Rep. *)
+(* Require Import VeriFFI.generator.Desc. *)
+(* Unset Strict Unquote Universe Mode. *)
 
-(** nat has to be representable *) 
-Variable nat_has: forall (g : graph) (n : nat) (v : VType), nat_in_graph g n (repNode v) -> graph_has_v g v.
+(* (** *** 4.0 Non-dependent, no indices/parameters - nat *) *)
+(* Set Printing All. *)
+(* Set Printing Universes. *)
+(* MetaCoq Run (in_graph_gen list). *)
+(* MetaCoq Run (in_graph_gen nat). *)
+(* Instance Rep_nat : Rep nat. rep_gen. Defined. *)
+(* MetaCoq Run (desc_gen O). *)
+(* MetaCoq Run (desc_gen S). *)
 
-Variable nat_monotone:   forall (g : graph) (to : nat) (lb : raw_vertex_block) (e : list (EType * (VType * VType)))
-    (n : nat) (p : rep_type),
-  add_node_compatible g (new_copied_v g to) e ->
-  graph_has_gen g to -> nat_in_graph g n p -> nat_in_graph (add_node g to lb e) n p.
+(* (** nat has to be representable *) *)
+(* Variable nat_has: forall (g : graph) (n : nat) (v : VType), nat_in_graph g n (repNode v) -> graph_has_v g v. *)
 
-Definition nat_representable: representable_X := 
-Build_representable_X nat nat_in_graph nat_has nat_monotone.
+(* Variable nat_monotone:   forall (g : graph) (to : nat) (lb : raw_vertex_block) (e : list (EType * (VType * VType))) *)
+(*     (n : nat) (p : rep_type), *)
+(*   add_node_compatible g (new_copied_v g to) e -> *)
+(*   graph_has_gen g to -> nat_in_graph g n p -> nat_in_graph (add_node g to lb e) n p. *)
 
-(** Constructor code  *) 
-Definition SucCode := 
-  ARG nat_representable (RES nat_representable).
+(* Definition nat_representable: representable_X := *)
+(* Build_representable_X nat nat_in_graph nat_has nat_monotone. *)
+
+(* (** Constructor code  *) *)
+(* Definition SucCode := *)
+(*   ARG nat_representable (RES nat_representable). *)
 
 
-(** *** 4.1 Parameters - Lists, cons 
+(** *** 4.1 Parameters - Lists, cons
 
-Specification we want: 
+Specification we want:
 
 Definition alloc_make_list_cons_spec : ident * funspec :=
-DECLARE _alloc_make_Coq_Init_Datatypes_list_cons 
+DECLARE _alloc_make_Coq_Init_Datatypes_list_cons
   WITH gv : globals, g : graph, p_x : rep_type, p_xs : rep_type, args : {graph_X_var : representable_X & (X_type graph_X_var (* x *) * list (X_type graph_X_var) (* xs *))%type },    roots : roots_t, sh : share, ti : val, outlier : outlier_t, f_info : fun_info, t_info : GCGraph.thread_info
-  PRE  [thread_info, tulong, tulong] 
+  PRE  [thread_info, tulong, tulong]
        PROP (X_in_graph (graph_X_var args) g (x args) p_x;
             list_in_graph (X_in_graph (graph_X_var args)) g (xs args) p_xs;
              writable_share sh
              )
-       PARAMS (ti; 
+       PARAMS (ti;
               rep_type_val g p_x;
               rep_type_val g p_xs)
        GLOBALS ()
-       SEP ( full_gc g t_info roots outlier ti sh ) 
-  POST [ tptr tulong ]  
-     EX (p' : rep_type) (g' : graph) (t_info' : GCGraph.thread_info), 
-     PROP (list_in_graph (X_in_graph (graph_X_var args)) g' ((x args) :: (xs args)) p'; 
+       SEP ( full_gc g t_info roots outlier ti sh )
+  POST [ tptr tulong ]
+     EX (p' : rep_type) (g' : graph) (t_info' : GCGraph.thread_info),
+     PROP (list_in_graph (X_in_graph (graph_X_var args)) g' ((x args) :: (xs args)) p';
            gc_graph_iso g roots g' roots
-         ) 
-     RETURN  (rep_type_val g' p')
-     SEP (full_gc g' t_info' roots outlier ti sh). 
-*) 
-
-(** 4.1.1 List has to be representable. *) 
-Parameter list_has : 
-forall X (g : graph) (n : list (X_type X)) (v : VType),
-   list_in_graph (X_in_graph X) g n (repNode v) -> graph_has_v g v.
-
-Parameter list_monotone : 
-forall X (g : graph) (to : nat) (lb : raw_vertex_block) (e : list (EType * (VType * VType)))
-     (n : list (X_type X)) (p : rep_type),
-   add_node_compatible g (new_copied_v g to) e ->
-   graph_has_gen g to ->
-   list_in_graph (X_in_graph X) g n p -> list_in_graph (X_in_graph X) (add_node g to lb e) n p.
-
-Definition list_representable_X (X : representable_X) : representable_X := 
-  Build_representable_X (list (X_type X)) (list_in_graph (X_in_graph X)) (list_has X) (list_monotone X). 
-
-(** Constructor code  *) 
-Definition consCode := 
-  TYPEPARAM (fun X => ARG X (ARG (list_representable_X X) (RES (list_representable_X X)))).
-
-(** Constructor description *)
-Definition consDescr : constructor_description.
-Proof.
-refine (Build_constructor_description _alloc_make_Coq_Init_Datatypes_list_cons consCode _).
-simpl. intros (X&x&xs&_). simpl. exact (x :: xs). 
-Defined.
-
-Definition nilCode :=
-  TYPEPARAM (fun X => RES (list_representable_X X)).
-
-Definition nilDescr : constructor_description.
-Proof.
-refine (Build_constructor_description _alloc_make_Coq_Init_Datatypes_list_cons nilCode _).
-simpl. intros (X&_). simpl. exact nil. 
-Defined.
-
-
-
-Definition graph_X_var  (args : {graph_X_var : representable_X & (X_type graph_X_var (* x *) * list (X_type graph_X_var) (* xs *))%type })  := let (graph_X_var, args') := args in graph_X_var. 
-
-Definition x (args : {graph_X_var : representable_X & (X_type graph_X_var (* x *) * list (X_type graph_X_var) (* xs *))%type }) : X_type (graph_X_var args). 
-Proof.
-  destruct args, p. exact x0.
-Defined.
-
-Definition xs (args : {graph_X_var : representable_X & (X_type graph_X_var (* x *) * list (X_type graph_X_var) (* xs *))%type }) : list (X_type (graph_X_var args)). 
-Proof.
-  destruct args, p. exact l.
-Defined.
-
-Definition alloc_make_list_cons_spec : ident * funspec :=
-DECLARE _alloc_make_Coq_Init_Datatypes_list_cons 
-  WITH gv : globals, g : graph, p_x : rep_type, p_xs : rep_type, args : {graph_X_var : representable_X & (X_type graph_X_var (* x *) * list (X_type graph_X_var) (* xs *))%type },    roots : roots_t, sh : share, ti : val, outlier : outlier_t, f_info : fun_info, t_info : GCGraph.thread_info
-  PRE  [thread_info, tulong, tulong] 
-       PROP (X_in_graph (graph_X_var args) g (x args) p_x;
-            list_in_graph (X_in_graph (graph_X_var args)) g (xs args) p_xs;
-             writable_share sh
-             )
-       PARAMS (ti; 
-              rep_type_val g p_x;
-              rep_type_val g p_xs)
-       GLOBALS ()
-       SEP ( full_gc g t_info roots outlier ti sh ) 
-  POST [ tptr tulong ]  
-     EX (p' : rep_type) (g' : graph) (t_info' : GCGraph.thread_info), 
-     PROP (list_in_graph (X_in_graph (graph_X_var args)) g' ((x args) :: (xs args)) p'; 
-           gc_graph_iso g roots g' roots
-         ) 
-     RETURN  (rep_type_val g' p')
-     SEP (full_gc g' t_info' roots outlier ti sh).  
-
-(** Definitional equality will be hard because of unit/all ps would have to be in a list.
- Probably, we'll want funspec_sub instead. *) 
-(* Lemma cons_same_spec :  alloc_make_list_cons_spec = alloc_make_spec_general consDescr.
-Proof.
-  unfold alloc_make_spec_general. simpl. 
-Admitted.
-
-Goal funspec_sub (snd (alloc_make_spec_general consDescr)) (snd alloc_make_list_cons_spec).
-Proof.
-  unfold funspec_sub.
-  simpl. intuition.
-Admitted. *)
-
-(** *** 4.2 Indices/silent arguments - Vector, cons *) 
-
-Inductive vector (A : Type) : nat -> Type :=
-   | vnil : vector A 0%nat 
-   | vcons : A -> forall n : nat, vector A n -> vector A (S n).
-
-(** 4.1.2 Vectors have to be representable - all this will be generated automatically. *)
-Variable _alloc_make_Coq_Init_Datatypes_vector_cons : ident.
-
-Variable vector_in_graph : forall X n, (graph -> X -> rep_type -> Prop) -> graph -> vector X n -> rep_type -> Prop.
-
-Variable vector_has :   forall X n (g : graph) (n0 : vector (X_type X) n) (v : VType),
-  vector_in_graph (X_type X) n (X_in_graph X) g n0 (repNode v) -> graph_has_v g v. 
-
-Variable vector_monotone : forall X n (g : graph) (to : nat) (lb : raw_vertex_block) (e : list (EType * (VType * VType)))
-   (n0 : vector (X_type X) n) (p : rep_type),
- add_node_compatible g (new_copied_v g to) e ->
- graph_has_gen g to ->
- vector_in_graph (X_type X) n (X_in_graph X) g n0 p ->
- vector_in_graph (X_type X) n (X_in_graph X) (add_node g to lb e) n0 p.
-
-Definition vector_representable_X (X : representable_X) (n :nat) : representable_X. 
-Proof. 
-  refine (Build_representable_X (vector (X_type X) n) (vector_in_graph (X_type X) n (X_in_graph X)) _ _).
-  - apply vector_has. 
-  - apply vector_monotone.
-Defined.
-
-(** Constructor code *) 
-Definition vectorConsCode := TYPEPARAM  (fun X => (ARG X (INDEX nat_representable (fun n => ARG (vector_representable_X X n) (RES (vector_representable_X X (S n))))))).
-
-(** Constructor description *)
-Definition vectorConsDescr : constructor_description.
-Proof.
-refine (Build_constructor_description _alloc_make_Coq_Init_Datatypes_list_cons vectorConsCode _).
-simpl. intros (X&x&n&xs&_). simpl. exact (vcons _ x n xs). 
-Defined.
-
-(** *** 4.3 Parameters and indices mixed -  param_and_index.
-
-The specification we'd want modulo a/b/pf being packed in a sigma type:
-
- Definition alloc_make_foo_spec : ident * funspec :=
-DECLARE _alloc_make_foo
-  WITH gv : globals, g : graph, a : nat, b: nat, pf : a < b, roots : roots_t, sh : share, ti : val, outlier : outlier_t, f_info : fun_info, t_info : GCGraph.thread_info
-  PRE  [thread_info, tulong] 
-       PROP (le_in_graph a b g pf p;
-             writable_share sh
-             )
-       PARAMS (ti; 
-              rep_type_val g p_x;
-              rep_type_val g p_xs)
-       GLOBALS ()
-       SEP ( full_gc g t_info roots outlier ti sh ) 
-  POST [ tptr tulong ]  
-     EX (p' : rep_type) (g' : graph) (t_info' : GCGraph.thread_info), 
-     PROP (param_and_index_in_graph a b pf g' (foo a b pf) p'; 
-           gc_graph_iso g roots g' roots
-         ) 
+         )
      RETURN  (rep_type_val g' p')
      SEP (full_gc g' t_info' roots outlier ti sh).
-*) 
+*)
 
-Inductive param_and_index (a b : nat) : (a < b)%nat -> Type :=
-| foo : forall (pf : (a < b)%nat), param_and_index a b pf.
+(** 4.1.1 List has to be representable. *)
+(* Parameter list_has : *)
+(* forall X (g : graph) (n : list (X_type X)) (v : VType), *)
+(*    list_in_graph (X_in_graph X) g n (repNode v) -> graph_has_v g v. *)
 
-Variable le_in_graph : forall (a b : nat), graph -> (a < b)%nat -> rep_type -> Prop.
+(* Parameter list_monotone : *)
+(* forall X (g : graph) (to : nat) (lb : raw_vertex_block) (e : list (EType * (VType * VType))) *)
+(*      (n : list (X_type X)) (p : rep_type), *)
+(*    add_node_compatible g (new_copied_v g to) e -> *)
+(*    graph_has_gen g to -> *)
+(*    list_in_graph (X_in_graph X) g n p -> list_in_graph (X_in_graph X) (add_node g to lb e) n p. *)
 
-Parameter le_has :   forall a b (g : graph) (n : (a < b)%nat) (v : VType),
-  le_in_graph a b g n (repNode v) -> graph_has_v g v.
+(* Definition list_representable_X (X : representable_X) : representable_X := *)
+(*   Build_representable_X (list (X_type X)) (list_in_graph (X_in_graph X)) (list_has X) (list_monotone X). *)
 
-Parameter le_c :  forall a b (g : graph) (to : nat) (lb : raw_vertex_block) (e : list (EType * (VType * VType)))
-    (n : (a < b)%nat) (p : rep_type),
-  add_node_compatible g (new_copied_v g to) e ->
-  graph_has_gen g to -> le_in_graph a b g n p -> le_in_graph a b (add_node g to lb e) n p.
+(* (** Constructor code  *) *)
+(* Definition consCode := *)
+(*   TYPEPARAM (fun X => ARG X (ARG (list_representable_X X) (RES (list_representable_X X)))). *)
 
-Definition le_representable (a b : nat) : representable_X.
-refine (Build_representable_X (a < b)%nat (le_in_graph a b) (le_has a b) (le_c a b)).
-Defined.
+(* (** Constructor description *) *)
+(* Definition consDescr : constructor_description. *)
+(* Proof. *)
+(* refine (Build_constructor_description _alloc_make_Coq_Init_Datatypes_list_cons consCode _). *)
+(* simpl. intros (X&x&xs&_). simpl. exact (x :: xs). *)
+(* Defined. *)
 
-Variable param_and_index_in_graph : forall (a b : nat) (pf : (a < b)%nat), graph -> param_and_index a b pf -> rep_type -> Prop.
+(* Definition nilCode := *)
+(*   TYPEPARAM (fun X => RES (list_representable_X X)). *)
 
-Variable param_and_index_has :   forall a b (lex : (a < b)%nat) (g : graph) (n : param_and_index a b lex) (v : VType),
-  param_and_index_in_graph a b lex g n (repNode v) -> graph_has_v g v. 
+(* Definition nilDescr : constructor_description. *)
+(* Proof. *)
+(* refine (Build_constructor_description _alloc_make_Coq_Init_Datatypes_list_cons nilCode _). *)
+(* simpl. intros (X&_). simpl. exact nil. *)
+(* Defined. *)
 
-Variable param_and_index_monotone:  forall a b (lex : (a < b)%nat) (g : graph) (to : nat) (lb : raw_vertex_block) (e : list (EType * (VType * VType)))
-   (n : param_and_index a b lex) (p : rep_type),
- add_node_compatible g (new_copied_v g to) e ->
- graph_has_gen g to ->
- param_and_index_in_graph a b lex g n p ->
- param_and_index_in_graph a b lex (add_node g to lb e) n p.
-
-Definition param_and_index_representable : forall  (a b : nat) (lex : (a < b)%nat), representable_X.
-Proof. 
-  intros a b lex. refine (Build_representable_X _ (param_and_index_in_graph a b lex) (param_and_index_has a b lex) (param_and_index_monotone a b lex)).
-Defined.
-
-(* Code for foo *)
-Definition param_and_indexCode :=
-  PARAM nat (fun a => PARAM nat (fun b => INDEX (le_representable a b) (fun pf => RES (param_and_index_representable a b pf) ) )). 
-
-Definition paramAndIndexDescr : constructor_description.
-Proof.
-  refine (Build_constructor_description  _alloc_make_Coq_Init_Datatypes_list_cons param_and_indexCode _).
-  simpl. intros (a&b&pf&_). simpl. exact (foo a b pf).
-Defined.
-
-(** 4.4 Dependent arguments - positive_nat_list
-
- Definition alloc_make_positive_nat_list_cons_spec : ident * funspec :=
-DECLARE _alloc_make_Coq_Init_Datatypes_list_cons 
-  WITH gv : globals, g : graph, x : nat, pf : 0 < x, xs : positive_nat_list,  roots : roots_t, sh : share, ti : val, outlier : outlier_t, f_info : fun_info, t_info : GCGraph.thread_info
-  PRE  [thread_info, tulong, tulong] 
-       PROP (nat_in_graph g x p_x; 
-             le_in_graph g pf p_pf;
-             positive_nat_list_in_graph g xs p_xs;
-             writable_share sh
-             )
-       PARAMS (ti; 
-              rep_type_val g p_x;
-              rep_type_val g p_xs)
-       GLOBALS ()
-       SEP ( full_gc g t_info roots outlier ti sh ) 
-  POST [ tptr tulong ]  
-     EX (p' : rep_type) (g' : graph) (t_info' : GCGraph.thread_info), 
-     PROP (positive_nat_list_in_graph g (pcons x pf xs) p'; 
-           gc_graph_iso g roots g' roots
-         ) 
-     RETURN  (rep_type_val g' p')
-     SEP (full_gc g' t_info' roots outlier ti sh). 
- *) 
-
-Inductive positive_nat_list : Type :=
-| pnil : positive_nat_list
-| pcons : forall (x : nat), (0 < x)%nat -> positive_nat_list -> positive_nat_list.
-
-Variable positive_nat_list_in_graph : graph -> positive_nat_list -> rep_type ->  Prop.
-
-Variable positive_nat_list_has: forall (g : graph) (n : positive_nat_list) (v : VType),
-  positive_nat_list_in_graph g n (repNode v) -> graph_has_v g v.
-
-Variable positive_nat_list_c: 
- forall (g : graph) (to : nat) (lb : raw_vertex_block) (e : list (EType * (VType * VType)))
-   (n : positive_nat_list) (p : rep_type),
- add_node_compatible g (new_copied_v g to) e ->
- graph_has_gen g to ->
- positive_nat_list_in_graph g n p -> positive_nat_list_in_graph (add_node g to lb e) n p.
-
-Definition positive_nat_list_representable : representable_X.
-refine (Build_representable_X _ positive_nat_list_in_graph positive_nat_list_has positive_nat_list_c).
-Defined.
-
-(* Code *) 
-Definition positve_nat_listCode := 
-  DEPARG nat_representable (fun x => ARG (le_representable 0 x) (ARG positive_nat_list_representable (RES positive_nat_list_representable))).
-
-(* Constructor description *) 
-Definition posNatListDescr : constructor_description.
-Proof.
-  refine (Build_constructor_description  _alloc_make_Coq_Init_Datatypes_list_cons positve_nat_listCode _).
-  simpl. intros (a&b&pf&_). exact (pcons a b pf).
-Defined.
+(* MetaCoq Run (in_graph_gen list). *)
+(* Instance Rep_list : forall A, Rep A -> Rep (list A). rep_gen. Defined. *)
+(* MetaCoq Run (desc_gen nil). *)
+(* MetaCoq Run (desc_gen cons). *)
 
 
+(* Definition graph_X_var  (args : {graph_X_var : representable_X & (X_type graph_X_var (* x *) * list (X_type graph_X_var) (* xs *))%type })  := let (graph_X_var, args') := args in graph_X_var. *)
 
+(* Definition x (args : {graph_X_var : representable_X & (X_type graph_X_var (* x *) * list (X_type graph_X_var) (* xs *))%type }) : X_type (graph_X_var args). *)
+(* Proof. *)
+(*   destruct args, p. exact x0. *)
+(* Defined. *)
 
+(* Definition xs (args : {graph_X_var : representable_X & (X_type graph_X_var (* x *) * list (X_type graph_X_var) (* xs *))%type }) : list (X_type (graph_X_var args)). *)
+(* Proof. *)
+(*   destruct args, p. exact l. *)
+(* Defined. *)
 
+(* Definition alloc_make_list_cons_spec : ident * funspec := *)
+(* DECLARE _alloc_make_Coq_Init_Datatypes_list_cons *)
+(*   WITH gv : globals, g : graph, p_x : rep_type, p_xs : rep_type, args : {graph_X_var : representable_X & (X_type graph_X_var (* x *) * list (X_type graph_X_var) (* xs *))%type },    roots : roots_t, sh : share, ti : val, outlier : outlier_t, f_info : fun_info, t_info : GCGraph.thread_info *)
+(*   PRE  [thread_info, tulong, tulong] *)
+(*        PROP (X_in_graph (graph_X_var args) g (x args) p_x; *)
+(*             list_in_graph (X_in_graph (graph_X_var args)) g (xs args) p_xs; *)
+(*              writable_share sh *)
+(*              ) *)
+(*        PARAMS (ti; *)
+(*               rep_type_val g p_x; *)
+(*               rep_type_val g p_xs) *)
+(*        GLOBALS () *)
+(*        SEP ( full_gc g t_info roots outlier ti sh ) *)
+(*   POST [ tptr tulong ] *)
+(*      EX (p' : rep_type) (g' : graph) (t_info' : GCGraph.thread_info), *)
+(*      PROP (list_in_graph (X_in_graph (graph_X_var args)) g' ((x args) :: (xs args)) p'; *)
+(*            gc_graph_iso g roots g' roots *)
+(*          ) *)
+(*      RETURN  (rep_type_val g' p') *)
+(*      SEP (full_gc g' t_info' roots outlier ti sh). *)
 
+(* (** Definitional equality will be hard because of unit/all ps would have to be in a list. *)
+(*  Probably, we'll want funspec_sub instead. *) *)
+(* (* Lemma cons_same_spec :  alloc_make_list_cons_spec = alloc_make_spec_general consDescr. *)
+(* Proof. *)
+(*   unfold alloc_make_spec_general. simpl. *)
+(* Admitted. *)
+
+(* Goal funspec_sub (snd (alloc_make_spec_general consDescr)) (snd alloc_make_list_cons_spec). *)
+(* Proof. *)
+(*   unfold funspec_sub. *)
+(*   simpl. intuition. *)
+(* Admitted. *) *)
+
+(* (** *** 4.2 Indices/silent arguments - Vector, cons *) *)
+
+(* Inductive vector (A : Type) : nat -> Type := *)
+(*    | vnil : vector A 0%nat *)
+(*    | vcons : A -> forall n : nat, vector A n -> vector A (S n). *)
+
+(* (** 4.1.2 Vectors have to be representable - all this will be generated automatically. *) *)
+(* Variable _alloc_make_Coq_Init_Datatypes_vector_cons : ident. *)
+
+(* Variable vector_in_graph : forall X n, (graph -> X -> rep_type -> Prop) -> graph -> vector X n -> rep_type -> Prop. *)
+
+(* Variable vector_has :   forall X n (g : graph) (n0 : vector (X_type X) n) (v : VType), *)
+(*   vector_in_graph (X_type X) n (X_in_graph X) g n0 (repNode v) -> graph_has_v g v. *)
+
+(* Variable vector_monotone : forall X n (g : graph) (to : nat) (lb : raw_vertex_block) (e : list (EType * (VType * VType))) *)
+(*    (n0 : vector (X_type X) n) (p : rep_type), *)
+(*  add_node_compatible g (new_copied_v g to) e -> *)
+(*  graph_has_gen g to -> *)
+(*  vector_in_graph (X_type X) n (X_in_graph X) g n0 p -> *)
+(*  vector_in_graph (X_type X) n (X_in_graph X) (add_node g to lb e) n0 p. *)
+
+(* Definition vector_representable_X (X : representable_X) (n :nat) : representable_X. *)
+(* Proof. *)
+(*   refine (Build_representable_X (vector (X_type X) n) (vector_in_graph (X_type X) n (X_in_graph X)) _ _). *)
+(*   - apply vector_has. *)
+(*   - apply vector_monotone. *)
+(* Defined. *)
+
+(* (** Constructor code *) *)
+(* Definition vectorConsCode := TYPEPARAM  (fun X => (ARG X (INDEX nat_representable (fun n => ARG (vector_representable_X X n) (RES (vector_representable_X X (S n))))))). *)
+
+(* (** Constructor description *) *)
+(* Definition vectorConsDescr : constructor_description. *)
+(* Proof. *)
+(* refine (Build_constructor_description _alloc_make_Coq_Init_Datatypes_list_cons vectorConsCode _). *)
+(* simpl. intros (X&x&n&xs&_). simpl. exact (vcons _ x n xs). *)
+(* Defined. *)
+
+(* (** *** 4.3 Parameters and indices mixed -  param_and_index. *)
+
+(* The specification we'd want modulo a/b/pf being packed in a sigma type: *)
+
+(*  Definition alloc_make_foo_spec : ident * funspec := *)
+(* DECLARE _alloc_make_foo *)
+(*   WITH gv : globals, g : graph, a : nat, b: nat, pf : a < b, roots : roots_t, sh : share, ti : val, outlier : outlier_t, f_info : fun_info, t_info : GCGraph.thread_info *)
+(*   PRE  [thread_info, tulong] *)
+(*        PROP (le_in_graph a b g pf p; *)
+(*              writable_share sh *)
+(*              ) *)
+(*        PARAMS (ti; *)
+(*               rep_type_val g p_x; *)
+(*               rep_type_val g p_xs) *)
+(*        GLOBALS () *)
+(*        SEP ( full_gc g t_info roots outlier ti sh ) *)
+(*   POST [ tptr tulong ] *)
+(*      EX (p' : rep_type) (g' : graph) (t_info' : GCGraph.thread_info), *)
+(*      PROP (param_and_index_in_graph a b pf g' (foo a b pf) p'; *)
+(*            gc_graph_iso g roots g' roots *)
+(*          ) *)
+(*      RETURN  (rep_type_val g' p') *)
+(*      SEP (full_gc g' t_info' roots outlier ti sh). *)
+(* *) *)
+
+(* Inductive param_and_index (a b : nat) : (a < b)%nat -> Type := *)
+(* | foo : forall (pf : (a < b)%nat), param_and_index a b pf. *)
+
+(* Variable le_in_graph : forall (a b : nat), graph -> (a < b)%nat -> rep_type -> Prop. *)
+
+(* Parameter le_has :   forall a b (g : graph) (n : (a < b)%nat) (v : VType), *)
+(*   le_in_graph a b g n (repNode v) -> graph_has_v g v. *)
+
+(* Parameter le_c :  forall a b (g : graph) (to : nat) (lb : raw_vertex_block) (e : list (EType * (VType * VType))) *)
+(*     (n : (a < b)%nat) (p : rep_type), *)
+(*   add_node_compatible g (new_copied_v g to) e -> *)
+(*   graph_has_gen g to -> le_in_graph a b g n p -> le_in_graph a b (add_node g to lb e) n p. *)
+
+(* Definition le_representable (a b : nat) : representable_X. *)
+(* refine (Build_representable_X (a < b)%nat (le_in_graph a b) (le_has a b) (le_c a b)). *)
+(* Defined. *)
+
+(* Variable param_and_index_in_graph : forall (a b : nat) (pf : (a < b)%nat), graph -> param_and_index a b pf -> rep_type -> Prop. *)
+
+(* Variable param_and_index_has :   forall a b (lex : (a < b)%nat) (g : graph) (n : param_and_index a b lex) (v : VType), *)
+(*   param_and_index_in_graph a b lex g n (repNode v) -> graph_has_v g v. *)
+
+(* Variable param_and_index_monotone:  forall a b (lex : (a < b)%nat) (g : graph) (to : nat) (lb : raw_vertex_block) (e : list (EType * (VType * VType))) *)
+(*    (n : param_and_index a b lex) (p : rep_type), *)
+(*  add_node_compatible g (new_copied_v g to) e -> *)
+(*  graph_has_gen g to -> *)
+(*  param_and_index_in_graph a b lex g n p -> *)
+(*  param_and_index_in_graph a b lex (add_node g to lb e) n p. *)
+
+(* Definition param_and_index_representable : forall  (a b : nat) (lex : (a < b)%nat), representable_X. *)
+(* Proof. *)
+(*   intros a b lex. refine (Build_representable_X _ (param_and_index_in_graph a b lex) (param_and_index_has a b lex) (param_and_index_monotone a b lex)). *)
+(* Defined. *)
+
+(* (* Code for foo *) *)
+(* Definition param_and_indexCode := *)
+(*   PARAM nat (fun a => PARAM nat (fun b => INDEX (le_representable a b) (fun pf => RES (param_and_index_representable a b pf) ) )). *)
+
+(* Definition paramAndIndexDescr : constructor_description. *)
+(* Proof. *)
+(*   refine (Build_constructor_description  _alloc_make_Coq_Init_Datatypes_list_cons param_and_indexCode _). *)
+(*   simpl. intros (a&b&pf&_). simpl. exact (foo a b pf). *)
+(* Defined. *)
+
+(* (** 4.4 Dependent arguments - positive_nat_list *)
+
+(*  Definition alloc_make_positive_nat_list_cons_spec : ident * funspec := *)
+(* DECLARE _alloc_make_Coq_Init_Datatypes_list_cons *)
+(*   WITH gv : globals, g : graph, x : nat, pf : 0 < x, xs : positive_nat_list,  roots : roots_t, sh : share, ti : val, outlier : outlier_t, f_info : fun_info, t_info : GCGraph.thread_info *)
+(*   PRE  [thread_info, tulong, tulong] *)
+(*        PROP (nat_in_graph g x p_x; *)
+(*              le_in_graph g pf p_pf; *)
+(*              positive_nat_list_in_graph g xs p_xs; *)
+(*              writable_share sh *)
+(*              ) *)
+(*        PARAMS (ti; *)
+(*               rep_type_val g p_x; *)
+(*               rep_type_val g p_xs) *)
+(*        GLOBALS () *)
+(*        SEP ( full_gc g t_info roots outlier ti sh ) *)
+(*   POST [ tptr tulong ] *)
+(*      EX (p' : rep_type) (g' : graph) (t_info' : GCGraph.thread_info), *)
+(*      PROP (positive_nat_list_in_graph g (pcons x pf xs) p'; *)
+(*            gc_graph_iso g roots g' roots *)
+(*          ) *)
+(*      RETURN  (rep_type_val g' p') *)
+(*      SEP (full_gc g' t_info' roots outlier ti sh). *)
+(*  *) *)
+
+(* Inductive positive_nat_list : Type := *)
+(* | pnil : positive_nat_list *)
+(* | pcons : forall (x : nat), (0 < x)%nat -> positive_nat_list -> positive_nat_list. *)
+
+(* Variable positive_nat_list_in_graph : graph -> positive_nat_list -> rep_type ->  Prop. *)
+
+(* Variable positive_nat_list_has: forall (g : graph) (n : positive_nat_list) (v : VType), *)
+(*   positive_nat_list_in_graph g n (repNode v) -> graph_has_v g v. *)
+
+(* Variable positive_nat_list_c: *)
+(*  forall (g : graph) (to : nat) (lb : raw_vertex_block) (e : list (EType * (VType * VType))) *)
+(*    (n : positive_nat_list) (p : rep_type), *)
+(*  add_node_compatible g (new_copied_v g to) e -> *)
+(*  graph_has_gen g to -> *)
+(*  positive_nat_list_in_graph g n p -> positive_nat_list_in_graph (add_node g to lb e) n p. *)
+
+(* Definition positive_nat_list_representable : representable_X. *)
+(* refine (Build_representable_X _ positive_nat_list_in_graph positive_nat_list_has positive_nat_list_c). *)
+(* Defined. *)
+
+(* (* Code *) *)
+(* Definition positve_nat_listCode := *)
+(*   DEPARG nat_representable (fun x => ARG (le_representable 0 x) (ARG positive_nat_list_representable (RES positive_nat_list_representable))). *)
+
+(* (* Constructor description *) *)
+(* Definition posNatListDescr : constructor_description. *)
+(* Proof. *)
+(*   refine (Build_constructor_description  _alloc_make_Coq_Init_Datatypes_list_cons positve_nat_listCode _). *)
+(*   simpl. intros (a&b&pf&_). exact (pcons a b pf). *)
+(* Defined. *)
