examples/verif.v
@@ -1,0 +1,15 @@
+Require Export VeriFFI.library.base_representation.
+Require Export VeriFFI.library.meta.
+Require Export VeriFFI.generator.InGraph.
+Require Export VeriFFI.generator.Rep.
+Require Export VeriFFI.generator.Desc.
+
+
+Unset Strict Unquote Universe Mode.
+
+MetaCoq Run (in_graph_gen nat).
+Instance Rep_nat : Rep nat. rep_gen. Defined.
+MetaCoq Run (desc_gen O).
+MetaCoq Run (desc_gen S).
+
+
