generator/Rep.v
@@ -1,0 +1,173 @@
+Require Import Coq.ZArith.ZArith
+               Coq.Program.Basics
+               Coq.Strings.String
+               Coq.Lists.List
+               Coq.Lists.ListSet.
+
+Require Import ExtLib.Structures.Monads
+               ExtLib.Data.Monads.OptionMonad
+               ExtLib.Data.Monads.StateMonad
+               ExtLib.Data.String.
+
+Require Import VeriFFI.generator.gen_utils.
+Require Import VeriFFI.library.base_representation.
+Require Import VeriFFI.library.meta.
+Require Import VeriFFI.generator.InGraph.
+
+(* Warning: MetaCoq doesn't use the Monad notation from ExtLib,
+  therefore don't expect ExtLib functions to work with TemplateMonad. *)
+Import ListNotations.
+
+Unset Strict Unquote Universe Mode.
+
+Ltac destruct_conj H :=
+  match type of H with
+  | @ex _ _ =>
+    let p := fresh "p" in
+    let m := fresh "M" in
+    destruct H as [p m]; destruct_conj m
+  | @and _ _ =>
+    let m1 := fresh "M" in
+    let m2 := fresh "M" in
+    destruct H as [m1 m2]; destruct_conj m2
+  | _ => idtac
+  end.
+
+Ltac prove_has_v :=
+  intros g x v;
+  destruct x; intros H; simpl in *;
+  try contradiction ; try (destruct_conj H; intuition).
+
+Ltac prove_monotone_with_IH :=
+  match goal with
+  | [IH : forall (_ : rep_type), _ |- _ ] =>
+    eapply IH; simpl; eauto
+  end.
+
+Ltac prove_monotone_with_IH' :=
+  match goal with
+  | [IH : forall (_ : @eq _ _ _) (_ : rep_type), _ |- _ ] =>
+    eapply IH; simpl; eauto
+  end.
+
+
+Axiom graph_cRep_add_node : forall g to lb e p ts ps,
+  add_node_compatible g (new_copied_v g to) e
+   -> graph_has_gen g to
+   -> graph_cRep g p ts ps
+   -> graph_cRep (add_node g to lb e) p ts ps.
+
+Ltac mon n :=
+  let i := fresh "i" in
+  match goal with
+  | [|- @is_in_graph _ _ _ n _] =>
+    let t := type of n in
+    epose (i := @is_monotone t _ _ _ _ _ _ _ _ _ _)
+  end;
+  eapply i.
+
+Ltac loop_over_app C :=
+  match C with
+  | ?a ?b =>
+    match a with
+    | ?c ?d => loop_over_app a ; mon d
+    | ?e => mon b
+    end
+  | _ => idtac
+  end.
+
+Ltac prove_monotone :=
+  intros g to lb e x p C G; revert p;
+  induction x;
+  unshelve (match goal with
+  | [|- forall _ _, @is_in_graph _ _ _ ?this _] =>
+    intros p H;
+    hnf in H;
+    destruct_conj H;
+    repeat eexists;
+    repeat split;
+    loop_over_app this;
+    try prove_monotone_with_IH;
+    try (eauto || (eapply graph_cRep_add_node; eauto))
+  end); auto.
+
+Ltac rep_gen :=
+  intros;
+  repeat (match goal with
+          | [R : Rep _ |- _] => destruct R
+          end);
+  econstructor; [prove_has_v | prove_monotone].
+
+(* MetaCoq Run (in_graph_gen list). *)
+(* Instance Rep_list : forall A `{Rep_A: Rep A}, Rep (list A). *)
+(*   rep_gen. *)
+(* Defined. *)
+
+(* MetaCoq Run (in_graph_gen nat). *)
+(* Instance Rep_nat : Rep nat. *)
+(*   rep_gen. *)
+(* Defined. *)
+
+(* MetaCoq Run (in_graph_gen bool). *)
+(* Instance Rep_bool : Rep bool. *)
+(* econstructor. *)
+(* prove_has_v. *)
+(* prove_monotone. *)
+(* Defined. *)
+
+(* Inductive T := *)
+(* | C1 : T *)
+(* | C2 : bool -> T *)
+(* | C3 : bool -> bool -> T -> T. *)
+
+(* MetaCoq Run (in_graph_gen T). *)
+(* Instance Rep_T : Rep T. *)
+(* econstructor. *)
+(* prove_has_v. *)
+(* prove_monotone. *)
+(* Defined. *)
+
+
+(* MetaCoq Run (in_graph_gen option). *)
+(* Definition Rep_option : forall A `{Rep_A: Rep A}, Rep (option A). *)
+(* intros. destruct Rep_A. *)
+(* econstructor. *)
+(* prove_has_v. *)
+(* prove_monotone. *)
+(* Defined. *)
+
+(* MetaCoq Run (in_graph_gen prod). *)
+(* Definition Rep_prod : forall A `{Rep_A: Rep A} B `{Rep_B : Rep B}, Rep (prod A B). *)
+(* intros. destruct Rep_A. destruct Rep_B. *)
+(* econstructor. *)
+(* prove_has_v. *)
+(* prove_monotone. *)
+(* Defined. *)
+
+
+(* Inductive vec (A : Type) : nat -> Type := *)
+(* | vnil : vec A O *)
+(* | vcons : forall n, A -> vec A n -> vec A (S n). *)
+(* MetaCoq Run (in_graph_gen vec). *)
+
+(* (* MetaCoq Run (in_graph_gen vec). *) *)
+(* Instance InGraph_vec (A : Type) (InGraph_A : InGraph A) (n : nat) : InGraph (vec A n) := *)
+(*   let fix is_in_graph_vec (n : nat) (g : graph) (x : vec A n) (p : rep_type) {struct x} : Prop := *)
+(*     match x with *)
+(*     | vnil => graph_cRep g p (enum 0) [] *)
+(*     | vcons arg0 arg1 arg2 => *)
+(*         exists p0 p1 p2 : rep_type, *)
+(*           @is_in_graph nat InGraph_nat g arg0 p0 /\ *)
+(*           @is_in_graph A InGraph_A g arg1 p1 /\ *)
+(*           is_in_graph_vec arg0 g arg2 p2 /\ *)
+(*           graph_cRep g p (boxed 0 3) [p0; p1; p2] *)
+(*     end *)
+(*     in @Build_InGraph (vec A n) (is_in_graph_vec n). *)
+
+(* Definition Rep_vec : forall A `{Rep_A: Rep A} n, Rep (vec A n). *)
+
+(* intros. destruct Rep_A. *)
+(* econstructor. *)
+(* prove_has_v. *)
+(* prove_monotone. *)
+(* Defined. *)
