generator/gen_utils.v
@@ -259,3 +259,278 @@ Module MetaCoqNotations.
     (only parsing).
   (* Compute <? option ?>. *)
 End MetaCoqNotations.
+
+From MetaCoq.Template Require Import BasicAst.
+Require Import MetaCoq.Template.All.
+
+(* Warning: MetaCoq doesn't use the Monad notation from ExtLib,
+  therefore don't expect ExtLib functions to work with TemplateMonad. *)
+Import monad_utils.MCMonadNotation
+       ListNotations
+       MetaCoqNotations.
+
+(* Alias to distinguish terms that are NOT in de Bruijn notation. *)
+Definition named_term : Type := term.
+(* Alias for terms that do not contain references to local variables,
+   therefore can be used in either [term]s in de Bruijn notation
+   and [named_term]s in named notation. *)
+Definition global_term : Type := term.
+(* Alias to denote that a function works with
+   either [term], [named_term] or [global_term]. *)
+Definition any_term : Type := term.
+
+Module DB.
+  (* Inspired by code written by John Li but changed slightly.
+     We should eventually consider making a MetaCoq_utils module. *)
+
+  (* Takes a named representation and converts it into the de Bruijn representation. *)
+  Definition deBruijn' (ctx : list name) (t : named_term) : TemplateMonad term :=
+    let fix find_in_ctx (count : nat) (id : BasicAst.ident) (ctx : list name) : option nat :=
+      match ctx with
+      | nil => None
+      | nAnon :: ns => find_in_ctx (S count) id ns
+      | (nNamed id') :: ns =>
+        if BasicAst.ident_eq id id' then Some count else find_in_ctx (S count) id ns
+      end in
+    let fix go (ctx : list name) (t : named_term) : TemplateMonad term :=
+        let go_mfix (mf : mfixpoint named_term) : TemplateMonad (mfixpoint term) :=
+          let ctx' := map (fun x => binder_name (dname x)) mf in
+          monad_map (fun def =>
+                       dtype' <- go ctx def.(dtype) ;;
+                       dbody' <- go (rev ctx' ++ ctx) def.(dbody) ;;
+                       ret (mkdef _ def.(dname) dtype' dbody' def.(rarg))) mf
+        in
+        match t with
+        | tRel n => ret t
+        | tVar id =>
+            match find_in_ctx O id ctx with
+            | Some i => ret (tRel i)
+            | None => ret t (* could be a free variable *)
+            end
+        | tEvar ev args =>
+            args' <- monad_map (go ctx) args ;;
+            ret (tEvar ev args')
+        | tSort s =>
+          ret t
+        | tCast t kind v =>
+            t' <- go ctx t ;;
+            v' <- go ctx v ;;
+            ret (tCast t' kind v')
+        | tProd na ty body =>
+            ty' <- go ctx ty ;;
+            body' <- go (binder_name na :: ctx) body ;;
+            ret (tProd na ty' body')
+        | tLambda na ty body =>
+            ty' <- go ctx ty ;;
+            body' <- go (binder_name na :: ctx) body ;;
+            ret (tLambda na ty' body')
+        | tLetIn na def def_ty body =>
+            def' <- go ctx def ;;
+            def_ty' <- go ctx def_ty ;;
+            body' <- go (binder_name na :: ctx) body ;;
+            ret (tLetIn na def' def_ty' body')
+        | tApp f args =>
+            f' <- go ctx f ;;
+            args' <- monad_map (go ctx) args ;;
+            ret (tApp f' args')
+        | tConst c u => ret t
+        | tInd ind u => ret t
+        | tConstruct ind idx u => ret t
+        | tCase ind_nbparams_relevance type_info discr branches =>
+            type_info' <- go ctx type_info ;;
+            discr' <- go ctx discr ;;
+            branches' <- monad_map (fun '(n, t) => t' <- go ctx t ;; ret (n, t')) branches ;;
+            ret (tCase ind_nbparams_relevance type_info' discr' branches')
+        | tProj proj t =>
+            t' <- go ctx t ;;
+            ret (tProj proj t')
+        | tFix mfix idx =>
+            mfix' <- go_mfix mfix ;;
+            ret (tFix mfix' idx)
+        | tCoFix mfix idx =>
+            mfix' <- go_mfix mfix ;;
+            ret (tCoFix mfix' idx)
+        | tInt p => ret (tInt p)
+        | tFloat p => ret (tFloat p)
+        end
+    in go ctx t.
+
+  Definition deBruijn (t : named_term) : TemplateMonad term := deBruijn' nil t.
+
+  (* Takes a de Bruijn representation and changes [tRel]s to [tVar]s. *)
+  Definition undeBruijn' (ctx : list name) (t : term) : TemplateMonad named_term :=
+    let fix go (ctx : list name) (t : term) : TemplateMonad named_term :=
+        let go_mfix (mf : mfixpoint term) : TemplateMonad (mfixpoint named_term) :=
+          let ctx' := map (fun x => binder_name (dname x)) mf in
+          monad_map (fun def =>
+                       dtype' <- go ctx def.(dtype) ;;
+                       dbody' <- go (rev ctx' ++ ctx) def.(dbody) ;;
+                       ret (mkdef _ def.(dname) dtype' dbody' def.(rarg))) mf
+        in
+        match t with
+        | tRel n =>
+            match nth_error ctx n with
+            | None => ret t
+            | Some nAnon => tmFail "Reference to anonymous binding"
+            | Some (nNamed id) => ret (tVar id)
+            end
+        | tVar id => ret t
+        | tEvar ev args =>
+            args' <- monad_map (go ctx) args ;;
+            ret (tEvar ev args')
+        | tSort s =>
+          ret t
+        | tCast t kind v =>
+            t' <- go ctx t ;;
+            v' <- go ctx v ;;
+            ret (tCast t' kind v')
+        | tProd na ty body =>
+            ty' <- go ctx ty ;;
+            body' <- go (binder_name na :: ctx) body ;;
+            ret (tProd na ty' body')
+        | tLambda na ty body =>
+            ty' <- go ctx ty ;;
+            body' <- go (binder_name na :: ctx) body ;;
+            ret (tLambda na ty' body')
+        | tLetIn na def def_ty body =>
+            def' <- go ctx def ;;
+            def_ty' <- go ctx def_ty ;;
+            body' <- go (binder_name na :: ctx) body ;;
+            ret (tLetIn na def' def_ty' body')
+        | tApp f args =>
+            f' <- go ctx f ;;
+            args' <- monad_map (go ctx) args ;;
+            ret (tApp f' args')
+        | tConst c u => ret t
+        | tInd ind u => ret t
+        | tConstruct ind idx u => ret t
+        | tCase ind_nbparams_relevance type_info discr branches =>
+            type_info' <- go ctx type_info ;;
+            discr' <- go ctx discr ;;
+            branches' <- monad_map (fun '(n, t) => t' <- go ctx t ;; ret (n, t')) branches ;;
+            ret (tCase ind_nbparams_relevance type_info' discr' branches')
+        | tProj proj t =>
+            t' <- go ctx t ;;
+            ret (tProj proj t')
+        | tFix mfix idx =>
+            mfix' <- go_mfix mfix ;;
+            ret (tFix mfix' idx)
+        | tCoFix mfix idx =>
+            mfix' <- go_mfix mfix ;;
+            ret (tCoFix mfix' idx)
+        | tInt p => ret (tInt p)
+        | tFloat p => ret (tFloat p)
+        end
+    in go ctx t.
+
+  Definition undeBruijn (t : term) : TemplateMonad named_term :=
+    undeBruijn' nil t.
+
+  (* Example usage for deBruijn:
+
+   MetaCoq Run (t <- DB.deBruijn
+                      (tLambda (mkBindAnn (nNamed "x") Relevant)
+                                <% bool %> (tVar "x"))%string ;;
+                t' <- tmUnquoteTyped (bool -> bool) t ;;
+                tmPrint t).
+  *)
+
+  (* Example usage for undeBruijn:
+
+   MetaCoq Run (t <- DB.undeBruijn <% fun (x : bool) => x %> ;;
+                tmPrint t).
+  *)
+
+  (* Round trip test:
+
+  MetaCoq Run (t <- DB.undeBruijn
+                      <% fix f (x y : nat) :=
+                           match x with S x' => f x' (S y) | O => y end %> ;;
+               t <- DB.deBruijn t ;;
+               t' <- tmUnquoteTyped (nat -> nat -> nat) t ;;
+               tmPrint t').
+  *)
+
+End DB.
+
+Module Substitution.
+  (* Capturing substitution for named terms, only use for global terms. *)
+  Fixpoint named_subst (t : global_term) (x : BasicAst.ident) (u : named_term) {struct u} : named_term :=
+    match u with
+    | tVar id => if eq_string id x then t else u
+    | tEvar ev args => tEvar ev (map (named_subst t x) args)
+    | tCast c kind ty => tCast (named_subst t x c) kind (named_subst t x ty)
+    | tProd (mkBindAnn (nNamed id) rel) A B =>
+      if eq_string x id
+      then tProd (mkBindAnn (nNamed id) rel) (named_subst t x A) B
+      else tProd (mkBindAnn (nNamed id) rel) (named_subst t x A) (named_subst t x B)
+    | tProd na A B => tProd na (named_subst t x A) (named_subst t x B)
+    | tLambda (mkBindAnn (nNamed id) rel) T M =>
+      if eq_string x id
+      then tLambda (mkBindAnn (nNamed id) rel) (named_subst t x T) M
+      else tLambda (mkBindAnn (nNamed id) rel) (named_subst t x T) (named_subst t x M)
+    | tLambda na T M => tLambda na (named_subst t x T) (named_subst t x M)
+    | tLetIn (mkBindAnn (nNamed id) rel) b ty b' =>
+      if eq_string x id
+      then tLetIn (mkBindAnn (nNamed id) rel) (named_subst t x b) (named_subst t x ty) b'
+      else tLetIn (mkBindAnn (nNamed id) rel) (named_subst t x b) (named_subst t x ty) (named_subst t x b')
+    | tLetIn na b ty b' => tLetIn na (named_subst t x b) (named_subst t x ty) (named_subst t x b')
+    | tApp u0 v => mkApps (named_subst t x u0) (map (named_subst t x) v)
+    | tCase ind p c brs =>
+        let brs' := map (on_snd (named_subst t x)) brs in
+        tCase ind (named_subst t x p) (named_subst t x c) brs'
+    | tProj p c => tProj p (named_subst t x c)
+    | tFix mfix idx => (* FIXME *)
+      let mfix' := map (map_def (named_subst t x) (named_subst t x)) mfix in
+      tFix mfix' idx
+    | tCoFix mfix idx =>
+      let mfix' := map (map_def (named_subst t x) (named_subst t x)) mfix in
+      tCoFix mfix' idx
+    | _ => u
+    end.
+
+  (* Substitute multiple [named_term]s into a [named_term]. *)
+  Fixpoint named_subst_all (l : list (BasicAst.ident * named_term)) (u : named_term) : named_term :=
+    match l with
+    | nil => u
+    | (id, t) :: l' => named_subst_all l' (named_subst t id u)
+    end.
+End Substitution.
+
+Module ConstSubstitution.
+  Fixpoint named_subst (t : global_term) (x : kername) (u : named_term) {struct u} : named_term :=
+    match u with
+    | tConst kn _ => if eq_kername x kn then t else u
+    | tVar id => t
+    | tEvar ev args => tEvar ev (map (named_subst t x) args)
+    | tCast c kind ty => tCast (named_subst t x c) kind (named_subst t x ty)
+    | tProd (mkBindAnn (nNamed id) rel) A B =>
+      tProd (mkBindAnn (nNamed id) rel) (named_subst t x A) (named_subst t x B)
+    | tProd na A B => tProd na (named_subst t x A) (named_subst t x B)
+    | tLambda (mkBindAnn (nNamed id) rel) T M =>
+      tLambda (mkBindAnn (nNamed id) rel) (named_subst t x T) (named_subst t x M)
+    | tLambda na T M => tLambda na (named_subst t x T) (named_subst t x M)
+    | tLetIn (mkBindAnn (nNamed id) rel) b ty b' =>
+      tLetIn (mkBindAnn (nNamed id) rel) (named_subst t x b) (named_subst t x ty) (named_subst t x b')
+    | tLetIn na b ty b' => tLetIn na (named_subst t x b) (named_subst t x ty) (named_subst t x b')
+    | tApp u0 v => mkApps (named_subst t x u0) (map (named_subst t x) v)
+    | tCase ind p c brs =>
+        let brs' := map (on_snd (named_subst t x)) brs in
+        tCase ind (named_subst t x p) (named_subst t x c) brs'
+    | tProj p c => tProj p (named_subst t x c)
+    | tFix mfix idx => (* FIXME *)
+      let mfix' := map (map_def (named_subst t x) (named_subst t x)) mfix in
+      tFix mfix' idx
+    | tCoFix mfix idx =>
+      let mfix' := map (map_def (named_subst t x) (named_subst t x)) mfix in
+      tCoFix mfix' idx
+    | _ => u
+    end.
+
+  (* Substitute multiple [named_term]s into a [named_term]. *)
+  Fixpoint named_subst_all (l : list (kername * named_term)) (u : named_term) : named_term :=
+    match l with
+    | nil => u
+    | (id, t) :: l' => named_subst_all l' (named_subst t id u)
+    end.
+End ConstSubstitution.
