library/meta.v
@@ -1,0 +1,227 @@
+Require Import Coq.ZArith.ZArith
+               Coq.Program.Basics
+               Coq.Strings.String
+               Coq.Lists.List
+               Coq.Lists.ListSet.
+
+Require Import ExtLib.Structures.Monads
+               ExtLib.Data.Monads.OptionMonad
+               ExtLib.Data.Monads.StateMonad
+               ExtLib.Data.String.
+
+From MetaCoq.Template Require Import BasicAst.
+Require Import MetaCoq.Template.All.
+
+Require Import VeriFFI.library.base_representation.
+
+(* Warning: MetaCoq doesn't use the Monad notation from ExtLib,
+  therefore don't expect ExtLib functions to work with TemplateMonad. *)
+Import ListNotations.
+
+From VeriFFI Require Export verification.graph_add.
+(* From VeriFFI Require Export verification.example.glue. *)
+(* From VeriFFI Require Export verification.specs_library. *)
+
+(* The type class to describe how a Coq type is represented in the CertiCoq heap graph.
+   We also have some lemmas about this representation as a part of the type class. *)
+Class InGraph (A : Type) :=
+  { is_in_graph : graph -> A -> rep_type -> Prop }.
+Class Rep (A : Type) : Type :=
+  { in_graph : InGraph A
+  ; has_v :
+      forall (g : graph) (n : A) (v : VType), is_in_graph g n (repNode v) -> graph_has_v g v
+  ; is_monotone :
+      forall (g : graph) (to : nat) (lb : raw_vertex_block)
+            (e : list (EType × VType × VType)) (n : A) (p : rep_type),
+      add_node_compatible g (new_copied_v g to) e ->
+      graph_has_gen g to -> is_in_graph g n p -> is_in_graph (add_node g to lb e) n p
+  }.
+
+(* Explain why we have type specific defs and proofs computed by tactics/metaprograms, instead of going from a deep embedded type desc to the proofs.  *)
+
+(* The type to represent a constructor in an inductive data type.
+   The name [reific] stands for "reified inductive constructor".
+   Notice how this type uses Gallina binders,
+   it is a weak HOAS description of the constructor. *)
+(* What other examples of cls are there? *)
+Inductive reific (cls : Type -> Type) : Type :=
+(* the type parameters in parametric polymorphism, isn't represented immediately in memory,
+but the possibility for representation is needed later, e.g., A in [list A] *)
+ | TYPEPARAM  : (forall (A : Type) `{cls A}, reific cls) -> reific cls
+(* Non-type parameters of a fixed type which isn't represented in memory, e.g., n in [n < m] *)
+ | PARAM  : forall A : Type, (A -> reific cls) -> reific cls
+(* index, represented in memory, e.g. the index of a vector *)
+ | INDEX  : forall (A : Type) `{cls A}, (A -> reific cls) ->reific cls
+ (* non-dependent version of arguments, argument represented in memory, e.g. for X/list X of cons *)
+ | ARG : forall (A : Type) `{cls A}, reific cls -> reific cls
+ (* dependent argument, represented in memory, e.g. in positive_nat_list *)
+ | DEPARG : forall (A : Type) `{cls A}, (A -> reific cls) -> reific cls
+(* the end type, e.g., list X for cons : forall X, X -> list X -> **list X** *)
+ | RES  : forall (A : Type) `{cls A}, reific cls.
+
+(* Makes nested sigmas (i.e. dependent tuples) of all the arguments. *)
+Fixpoint args {cls : Type -> Type} (c : reific cls) : Type :=
+  match c with
+  | TYPEPARAM f => {A : Type & {H : cls A & args (f A H)}}
+  | PARAM A f => {a : A & args (f a) }
+  | INDEX A H f => {a : A & args (f a)}
+  | ARG A H c => (A * args c)%type
+  | DEPARG A H f => {a : A & args (f a)}
+  | RES _ _ => unit
+  end.
+
+(* Instance of result type *)
+Fixpoint result {cls : Type -> Type} (c : reific cls) (xs : args c) : {A : Type & cls A} :=
+  match c as l return (args l -> {A : Type & cls A}) with
+  | TYPEPARAM f => fun P => let '(a; (h; rest)) := P in result (f a h) rest
+  | PARAM A f => fun P => let '(a; rest) := P in result (f a) rest
+  | INDEX A H f => fun P => let '(a; rest) := P in result (f a) rest
+  | ARG A H c => fun P => let '(a, rest) := P in result c rest
+  | DEPARG A H f => fun P => let '(a; rest) := P in result (f a) rest
+  | RES A H => fun _ => (A; H)
+  end xs.
+
+(* Makes a Coq level constructor type from a [reific], with the new type
+   taking a nested dependent tuple instead of curried arguments. *)
+Definition reconstruct {cls : Type -> Type} (c : reific cls) : Type :=
+  forall (P : args c),
+  projT1 (result c P).
+
+(* The same thing as [reconstruct] but takes the actual constructor
+   as an argument but "ignores" it. In reality that argument is
+   used by the tactic to infer how to reconstruct. *)
+Definition reconstructor {cls : Type -> Type} {T : Type} (x : T) (c : reific cls) :=
+  reconstruct c.
+
+Ltac destruct_through C :=
+  match goal with
+  | [P : (@sigT (_ _) _) |- _ ] =>
+    destruct P; destruct_through C
+  | [P : (@sigT _ _) |- _ ] =>
+    let a := fresh "a" in destruct P as [a];
+    destruct_through constr:(C a)
+  | [P : (@prod _ _) |- _ ] =>
+    let a := fresh "a" in destruct P as [a];
+    let C' := constr:(C a) in
+    destruct_through constr:(C a)
+  | [P : unit |- _ ] => exact C
+  end.
+
+Ltac reconstructing_aux C :=
+  let P := fresh "P" in
+  intro P;
+  simpl in P;
+  destruct_through C.
+
+(* The entry point to the tactic that solves
+   goals like [reconstructor S S_reific]. *)
+Ltac reconstructing :=
+  match goal with
+  | [ |- @reconstructor _ _ ?C _ ] => hnf; reconstructing_aux C
+  end.
+
+(* EXAMPLES *)
+(*
+Instance Rep_unit : Rep unit.
+  constructor. intros. exact True. Defined.
+Instance Rep_nat : Rep nat.
+  constructor. intros. exact True. Defined.
+Instance Rep_list : forall A : Type, Rep A -> Rep (list A).
+  intros. constructor. intros. exact True. Defined.
+
+Inductive vec (A : Type) : nat -> Type :=
+| vnil : vec A 0
+| vcons : forall n : nat, A -> vec A n -> vec A (S n).
+
+Check <%% vec %%>.
+Instance Rep_vec : forall (A : Type) (n : nat), Rep A -> Rep (vec A n).
+  intros. constructor. intros. exact True. Defined.
+
+Definition S_reific : reific :=
+  @ARG nat Rep_nat (@RES nat Rep_nat).
+Set Printing Universes.
+
+Polymorphic Inductive plist (A : Type) :=
+| pnil : plist A
+| pcons : A -> plist A -> plist A.
+Check <%% plist %%>.
+Polymorphic Cumulative Inductive pprod (A B : Type) :=
+| ppair : A -> B -> pprod A B.
+Check <%% @pprod %%>.
+Check tSort.
+
+Instance Rep_plist (A : Type) (Rep_A : Rep A) : Rep (plist A) :=
+  {| rep _ _ _ := False |}.
+
+Definition pcons_reific : reific :=
+  @TYPEPARAM (fun A H =>
+                @ARG A H
+                     (@ARG (plist A) (Rep_plist A H)
+                           (@RES (plist A) (Rep_plist A H)))).
+
+Definition pcons' : reconstructor (@pcons) pcons_reific.
+  reconstructing. Defined.
+Print pcons'.
+
+Check <%
+  @TYPEPARAM (fun A H =>
+                @ARG A H
+                     (@ARG (plist A) (Rep_plist A H)
+                           (@RES (plist A) (Rep_plist A H))))  %>.
+
+
+Definition cons_reific : reific :=
+  @TYPEPARAM (fun A H =>
+                @ARG A H
+                     (@ARG (list A) (Rep_list A H)
+                           (@RES (list A) (Rep_list A H)))).
+
+Compute reconstructor (@cons) cons_reific.
+Goal reconstructor (@cons) cons_reific.
+  reconstructing. Defined.
+
+Inductive two (A : Type) : Type :=
+| mkTwo : A -> A -> two A.
+
+Definition Rep_two : forall (A : Type), Rep A -> Rep (two A).
+  intros. constructor. intros. exact True. Defined.
+Existing Instance Rep_two.
+
+Definition mkTwo_reific : reific :=
+  @TYPEPARAM (fun A H =>
+                @ARG A H (@ARG A H (@RES (two A) (Rep_two A H)))).
+
+Goal reconstructor mkTwo mkTwo_reific.
+  reconstructing. Defined.
+
+Definition vnil_reific : reific :=
+  @TYPEPARAM (fun A H =>
+                (@RES (vec A O) (Rep_vec A O H))).
+
+Goal (reconstructor vnil vnil_reific).
+  reconstructing. Defined.
+
+Definition vcons_reific : reific :=
+  @TYPEPARAM (fun A H =>
+     @INDEX nat Rep_nat (fun n =>
+       @ARG A H (@ARG (vec A n) (Rep_vec A n H)
+          (@RES (vec A (S n)) (Rep_vec A (S n) H))))).
+
+Goal (reconstructor vcons vcons_reific).
+  reconstructing. Defined.
+
+Check <%% vec %%>.
+
+*)
+
+(* GENERATION *)
+Record constructor_description :=
+{ ctor_name : BasicAst.ident;
+  ctor_reific : reific Rep;
+  ctor_real : reconstruct ctor_reific
+}.
+
+Class Desc {T : Type} (ctor_val : T) :=
+  { desc : constructor_description }.
+
+Definition Reppyish := option ({A : Type & Rep A}).
